Owl/constants.v
@@ -1,7 +1,9 @@
 Record Lattice := {
   labels : Set;
-  leq : labels -> labels -> bool
+  leq : labels -> labels -> bool;
   bot : labels;
+  join : labels -> labels -> labels;
+  meet : labels -> labels -> labels;
 }.
 
 Axiom L : Lattice. 
